immutable-btree/BtreeImpl.dfy
@@ -1,0 +1,66 @@
+include "../lib/total_order.dfy"
+include "../lib/map_utils.dfy"
+include "../lib/mathematics.dfy"
+include "../lib/sequences.dfy"
+include "BtreeSpec.dfy"
+include "BtreeInv.dfy"
+
+abstract module BtreeImpl {
+  import Keyspace = Bounded_Total_Order
+  import opened BtreeSpec
+  import opened BtreeInv
+
+  lemma strictlySortedInsert(l: seq<Key>, k: Key, pos: int)
+  requires -1 <= pos < |l|;
+  requires Keyspace.IsStrictlySorted(l);
+  requires Keyspace.IsSorted(l);
+  requires pos == Keyspace.LargestLte(l, k);
+  requires pos < 0 || k != l[pos]
+  ensures Keyspace.IsStrictlySorted(l[..pos+1] + [k] + l[pos+1..]);
+  {
+    var l' := l[..pos+1] + [k] + l[pos+1..];
+    Keyspace.reveal_IsStrictlySorted();
+
+    forall i, j | 0 <= i < j < |l'|
+    ensures Keyspace.lt(l'[i], l'[j])
+    {
+    }
+  }
+
+  method put<Value>(tree: Node, key: Key, value: Value)
+  returns (newtree: Node)
+  requires WFTree(tree)
+  requires Keyspace.lte(tree.lb, key);
+  requires Keyspace.lt(key, tree.ub);
+  ensures Put(Constants(), Variables(tree), Variables(newtree), key, value)
+  decreases tree
+  {
+    if (tree.Leaf?) {
+      Keyspace.IsStrictlySortedImpliesIsSorted(tree.keys);
+      var pos := Keyspace.LargestLte(tree.keys, key);
+      if (pos >= 0 && key == tree.keys[pos]) {
+        return Leaf(tree.keys, tree.values[pos := value], tree.lb, tree.ub);
+      } else {
+        var newkeys := tree.keys[..pos+1] + [key] + tree.keys[pos+1..];
+        var newvals := tree.values[..pos+1] + [value] + tree.values[pos+1..];
+        return Leaf(newkeys, newvals, tree.lb, tree.ub);
+      }
+    } else {
+      Keyspace.IsStrictlySortedImpliesIsSorted(tree.pivots);
+      var pos := Keyspace.LargestLte(tree.pivots, key) + 1;
+
+      if (pos == 0) {
+        assert tree.children[pos].lb == tree.lb;
+        assert Keyspace.lte(tree.lb, key);
+      } else { 
+        assert tree.children[pos].lb == tree.pivots[pos-1];
+        assert Keyspace.lte(tree.pivots[pos-1], key);
+      }
+
+      var new_child := put(tree.children[pos], key, value);
+      var new_children := tree.children[pos := new_child];
+      return Index(tree.pivots, new_children, tree.lb, tree.ub);
+    }
+  }
+
+}
